CCsub_Substitution.v
@@ -50,7 +50,7 @@ Proof with simpl_env;
     simpl.
     destruct (X == Z); subst.
     + apply (sub_transitivity Q)...
-      * rewrite_env (nil ++ (EnvImpl.map (subst_tb Z P) Δ) ++ Γ).
+      * rewrite_env (nil ++ (map (subst_tb Z P) Δ) ++ Γ).
         apply sub_weakening...
       * rewrite (subst_tt_fresh Z P Q).
         2: {
@@ -60,51 +60,44 @@ Proof with simpl_env;
         }
         (* analyze_binds_uniq H... *)
         (* binds_get H. *)
-        apply EnvImpl.binds_app_1 in H...
+        apply binds_app_1 in H...
         destruct H...
-        { exfalso. epose proof (EnvImpl.binds_dom_contradiction)... }
-        apply EnvImpl.binds_app_1 in H...
+        { exfalso. epose proof binds_dom_contradiction... }
+        apply binds_app_1 in H...
         destruct H...
-        apply EnvImpl.binds_one_2 in H...
+        apply binds_one_2 in H...
         inversion H; subst.
         apply (IHSsubT Q)...
-        { exfalso. epose proof (EnvImpl.binds_dom_contradiction)... }
-    + EnvImpl.analyze_binds H...
-      * assert (EnvImpl.binds X (bind_sub U) (EnvImpl.map (subst_tb Z P) Δ ++ Γ)) by admit.
+        exfalso. epose proof binds_dom_contradiction...
+    + analyze_binds H...
+      * apply (sub_trans_tvar (subst_tt Z P U)); [auto | eapply IHSsubT]...
+      * 
+        (* assert (binds X (bind_sub U) (map (subst_tb Z P) Δ ++ Γ)) by admit. *)
         apply (sub_trans_tvar U)...
         rewrite (subst_tt_fresh Z P U).
         2: {
-          assert (wf_typ Γ S U) as HA. {
-            eapply wf_typ_from_binds_sub...
-            admit.
-          }
+          assert (wf_typ Γ S U) as HA by (eapply wf_typ_from_binds_sub; eauto).
           lets: notin_fv_wf_typ Z HA.
           fsetdec.
         }
         apply (IHSsubT Q)...
-      * apply (sub_trans_tvar (subst_tt Z P U)); [auto | eapply IHSsubT]...
-  - Case "sub_capt".
-    simpl; apply sub_capt...
-  - Case "sub_top".
-    simpl; apply sub_top...
-  - Case "sub_arr".
-    simpl; pick fresh y and apply sub_arr...
+  - simpl; apply sub_capt...
+  - simpl; apply sub_top...
+  - simpl; pick fresh y and apply sub_arr...
     repeat rewrite subst_tt_open_ct_var...
-    rewrite <- concat_assoc.
-    replace ([(y, bind_typ (C2 # subst_tt Z P R2))] ++ map (subst_tb Z P) Δ)
+    rewrite <- app_assoc.
+    replace ((y ~ bind_typ (C2 # subst_tt Z P R2) ++ map (subst_tb Z P) Δ))
        with (map (subst_tb Z P) ([(y, bind_typ (C2 # R2))] ++ Δ))
          by reflexivity.
     eapply H3...
-  - Case "sub_all".
-    simpl; pick fresh Y and apply sub_all...
+  - simpl; pick fresh Y and apply sub_all...
     repeat rewrite subst_tt_open_tt_var...
-    rewrite <- concat_assoc.
-    replace ([(Y, bind_sub (subst_tt Z P R2))] ++ map (subst_tb Z P) Δ)
+    rewrite <- app_assoc.
+    replace ((Y ~ bind_sub (subst_tt Z P R2) ++ map (subst_tb Z P) Δ))
        with (map (subst_tb Z P) ([(Y, bind_sub R2)] ++ Δ))
          by reflexivity.
     eapply H2...
-  - Case "sub_box".
-    simpl; apply sub_box...
+  - simpl; apply sub_box...
 Qed.
 
 Lemma sub_through_subst_ct : forall x CU U C Γ Δ R T S,
@@ -119,19 +112,18 @@ Proof with eauto using wf_ctx_subst_cb,
   remember (Δ ++ [(x, bind_typ (CU # U))] ++ Γ).
   generalize dependent Δ.
   induction Sub; intros Δ EQ; subst.
-  - Case "sub_refl_tvar".
-    apply sub_refl_tvar...
+  - apply sub_refl_tvar...
     inversion H0; subst...
     rename select (binds X _ _) into Binds.
-    binds_cases Binds...
+    analyze_binds Binds...
     apply wf_typ_var with (T := subst_ct x C T).
     replace (bind_sub (subst_ct x C T))
        with (subst_cb x C (bind_sub T))
          by reflexivity.
-    apply binds_head, binds_map; assumption.
-  - Case "sub_trans_tvar".
-    rename select (binds _ _ _) into Binds.
-    binds_cases Binds.
+    apply binds_app_2, binds_map; assumption.
+  - rename select (binds _ _ _) into Binds.
+    analyze_binds Binds.
+    + apply sub_trans_tvar with (U := subst_ct x C U0)...
     + apply sub_trans_tvar with (U := U0)...
       rewrite (subst_ct_fresh x C U0)...
       assert (WfCtx : wf_ctx (Δ ++ [(x, bind_typ (CU # U))] ++ Γ) S) by (applys sub_regular Sub).
@@ -141,32 +133,26 @@ Proof with eauto using wf_ctx_subst_cb,
       { applys wf_typ_ctx_bind_sub... }
       pose proof (notin_fv_wf_typ Γ x U0 S WfU0 ltac:(assumption)).
       fsetdec.
-    + apply sub_trans_tvar with (U := subst_ct x C U0)...
-  - Case "sub_capt".
-    apply sub_capt...
-  - Case "sub_top".
-    apply sub_top...
+  - apply sub_capt...
+  - apply sub_top...
     eapply wf_typ_subst_cb...
-  - Case "sub_arr".
-    pick fresh y and apply sub_arr...
+  - pick fresh y and apply sub_arr...
     fold subst_ct.
     repeat rewrite subst_ct_open_ct_var...
-    rewrite <- concat_assoc.
+    rewrite <- app_assoc.
     replace ([(y, bind_typ (subst_cse x C C2 # subst_ct x C R2))] ++ map (subst_cb x C) Δ)
        with (map (subst_cb x C) ([(y, bind_typ (C2 # R2))] ++ Δ))
          by reflexivity.
     eauto.
-  - Case "sub_all".
-    pick fresh Y and apply sub_all...
+  - pick fresh Y and apply sub_all...
     fold subst_ct.
     repeat rewrite subst_ct_open_tt_var...
-    rewrite <- concat_assoc.
+    rewrite <- app_assoc.
     replace ([(Y, bind_sub (subst_ct x C R2))] ++ map (subst_cb x C) Δ)
        with (map (subst_cb x C) ([(Y, bind_sub R2)] ++ Δ))
          by reflexivity.
-    eauto*.
-  - Case "sub_box".
-    apply sub_box.
+    eauto.
+  - apply sub_box.
     fold subst_ct.
     apply IHSub...
 Qed.
@@ -174,7 +160,7 @@ Qed.
 Lemma wf_pretyp_from_wf_ctx_typ : forall x C P Γ S,
   wf_ctx ([(x, bind_typ (C # P))] ++ Γ) S ->
   wf_typ Γ S (C # P).
-Proof with eauto*.
+Proof with eauto.
   intros * WfCtx.
   inversion WfCtx; auto; subst.
 Qed.
@@ -226,7 +212,7 @@ Lemma typing_through_subst_ve : forall Γ Δ x T C R e (u : atom) S,
   typing (Δ ++ [(x, bind_typ (C # R))] ++ Γ) S e T ->
   typing Γ S u (C # R) ->
   typing (map (subst_cb x (cse_fvar u)) Δ ++ Γ) S (subst_ve x u (cse_fvar u) e) (subst_ct x (cse_fvar u) T).
-Proof with eauto*.
+Proof with eauto.
   intros * Typ uTyp.
   forwards (WfStore & WfCtx & _ & WfT): typing_regular Typ.
   assert (WfCtx' : wf_ctx Γ S) by (repeat apply wf_ctx_tail in WfCtx; assumption).
@@ -236,7 +222,10 @@ Proof with eauto*.
     by (eapply wf_cse_from_binds; eauto).
   assert (WfCtxSubst : wf_ctx (map (subst_cb x (cse_fvar u)) Δ ++ Γ) S) by (eapply wf_ctx_subst_cb; eauto).
   assert (uNotInΔ : u ∉ dom Δ).
-  { eapply tail_not_in_head...
+  { apply uniq_from_wf_ctx in WfCtx.
+    apply uniq_app_3 in WfCtx.
+    unfold disjoint in WfCtx.
+    simpl in WfCtx.
     apply binds_In in Binds.
     simpl; fsetdec.
   }
@@ -245,14 +234,14 @@ Proof with eauto*.
   assert (xNotInQ : x ∉ fv_ct Q) by (eapply wf_typ_notin_fv_ct; eauto).
   assert (xNotInR : x ∉ fv_ct R) by (eapply wf_typ_notin_fv_ct; eauto).
   dependent induction Typ; simpl.
-  - Case "typing_var".
-    destruct (x0 == x); subst; try (exfalso; fsetdec).
-    + SCase "x0 = x".
-      rename select (binds x _ _) into Binds'.
-      binds_cases Binds'.
-      * exfalso; simpl in *; fsetdec.
+  - destruct (x0 == x); subst; try (exfalso; fsetdec).
+    + rename select (binds x _ _) into Binds'.
+      analyze_binds Binds'.
+      * rename select (binds x _ _) into Binds'.
+        apply binds_In in Binds'.
+        contradiction.
       * inversion select (bind_typ _ = bind_typ _); subst.
-        rewrite_nil_concat.
+        rewrite_env (nil ++ (map (subst_cb x (cse_fvar u)) Δ) ++ Γ).
         eapply typing_weakening.
         2: assumption.
         apply typing_sub with (R := cse_fvar u # R); simpl in *...
@@ -260,32 +249,29 @@ Proof with eauto*.
         inversion uTyp...
         apply sub_capt...
         -- rewrite <- subst_ct_fresh...
+           apply sub_reflexivity...
         -- rewrite <- subst_ct_fresh...
         -- rewrite <- subst_ct_fresh. apply sub_reflexivity...
            auto.
-      * rename select (binds x _ _) into Binds'.
-        apply binds_In in Binds'.
-        contradiction.
-    + SCase "x0 <> x".
-      rename select (binds x0 _ _) into Binds'.
-      binds_cases Binds'; destruct (x == x0); subst; simpl; destruct (x0 == x0); try fsetdec.
-      * destruct (x0 == x); destruct (x == x0); try fsetdec; simpl.
-        eapply typing_var with (C := C0)...
-        apply binds_tail...
-        rewrite <- subst_ct_fresh...
-        eapply wf_typ_notin_fv_ct with (Γ := Γ)...
-        rename select (binds x0 _ _) into Binds'.
-        destruct (wf_typ_ctx_bind_typ _ _ _ _ WfCtx' Binds') as [D0 [Q0 [Eq WfD0Q0]]]; inversion Eq; subst; clear Eq.
-        inversion WfD0Q0; subst...
+      * exfalso. apply binds_In in BindsTac0; fsetdec.
+    + rename select (binds x0 _ _) into Binds'.
+      analyze_binds Binds'; destruct (x == x0); subst; simpl; destruct (x0 == x0); try fsetdec.
       * destruct (x0 == x); destruct (x == x0); try fsetdec; simpl.
         eapply typing_var with (C := subst_cse x (cse_fvar u) C0)...
         rename select (binds x0 _ _) into Binds'.
         replace (bind_typ (subst_cse x (cse_fvar u) C0 # subst_ct x (cse_fvar u) R0))
            with (subst_cb x (cse_fvar u) (bind_typ (C0 # R0)))
              by reflexivity.
-        apply binds_head, binds_map, Binds'.
-  - Case "typing_abs".
-    rewrite subst_cse_cv_commutes_with_subst_ve.
+        apply binds_app_2, binds_map, Binds'.
+      * destruct (x0 == x); destruct (x == x0); try fsetdec; simpl.
+        eapply typing_var with (C := C0)...
+        apply binds_app_3...
+        rewrite <- subst_ct_fresh...
+        eapply wf_typ_notin_fv_ct with (Γ := Γ)...
+        rename select (binds x0 _ _) into Binds'.
+        destruct (wf_typ_ctx_bind_typ _ _ _ _ WfCtx' Binds') as [D0 [Q0 [Eq WfD0Q0]]]; inversion Eq; subst; clear Eq.
+        inversion WfD0Q0; subst...
+  - rewrite subst_cse_cv_commutes_with_subst_ve.
     pick fresh y and apply typing_abs.
     + replace (subst_cse x (cse_fvar u) C0 # subst_ct x (cse_fvar u) R0)
          with (subst_ct x (cse_fvar u) (C0 # R0))
@@ -300,15 +286,13 @@ Proof with eauto*.
       rewrite subst_ve_open_ve_var.
       2-3: auto.
       rename select (forall x0 : atom, x0 ∉ L -> forall (Γ0 Δ0 : ctx), _) into IH.
-      eapply IH with (C1 := C) (R1 := R)...
+      eapply IH with (C := C) (R := R)...
       eapply wf_ctx_subst_cb...
-  - Case "typing_app".
-    assert (Iff : (if f == x then (var_f u) else (var_f f)) = var_f (if f == x then u else f))
-      by (destruct_if; reflexivity).
+  - assert (Iff : (if f == x then (var_f u) else (var_f f)) = var_f (if f == x then u else f))
+      by (destruct (f == x); eauto).
     rewrite Iff.
     destruct (x0 == x); subst.
-    + SCase "x0 = x".
-      unfold open_ct.
+    + unfold open_ct.
       rewrite subst_ct_open_rec...
       simpl. simpl. destruct (x == x); try fsetdec...
       eapply typing_app.
@@ -322,8 +306,7 @@ Proof with eauto*.
            with (subst_ve x u (cse_fvar u) (exp_var (var_f x))).
         eapply IHTyp2...
         simpl; destruct (x == x); try fsetdec.
-    + SCase "x0 <> x".
-      rewrite <- subst_ct_open_ct_var...
+    + rewrite <- subst_ct_open_ct_var...
       apply typing_app with (D := subst_cse x (cse_fvar u) D) (Q := subst_ct x (cse_fvar u) Q) (C := subst_cse x (cse_fvar u) C0) (T := subst_ct x (cse_fvar u) T).
       * replace (subst_cse x (cse_fvar u) C0 # ∀ ((subst_cse x (cse_fvar u) D # subst_ct x (cse_fvar u) Q)) subst_ct x (cse_fvar u) T)
            with (subst_ct x (cse_fvar u) (C0 # ∀ (D # Q) T))
@@ -336,8 +319,7 @@ Proof with eauto*.
         erewrite subst_ve_fresh with (x := x) (u := u) (c := cse_fvar u) (e := x0).
         2: simpl; fsetdec.
         eapply IHTyp2...
-  - Case "typing_let".
-    pick fresh y and apply typing_let.
+  - pick fresh y and apply typing_let.
     + eapply IHTyp...
     + rewrite subst_ve_open_ve_var...
       fold subst_ct.
@@ -347,13 +329,12 @@ Proof with eauto*.
       rename select (forall x0 : atom, x0 ∉ L -> forall (Γ0 Δ0 : ctx), _) into IH.
       eapply IH...
       * apply wf_ctx_typ...
-      * rewrite concat_assoc.
+      * rewrite app_assoc.
         apply wf_typ_weaken_head.
         assumption. constructor...
       * eapply wf_ctx_subst_cb...
         eapply wf_ctx_typ...
-  - Case "typing_tabs".
-    rewrite subst_cse_cv_commutes_with_subst_ve.
+  - rewrite subst_cse_cv_commutes_with_subst_ve.
     pick fresh Y and apply typing_tabs.
     + eapply wf_typ_subst_cb...
     + apply subst_ct_pure_type...
@@ -368,9 +349,8 @@ Proof with eauto*.
       rename select (forall X : atom, X ∉ L -> forall (Γ0 Δ0 : ctx), _) into IH.
       eapply IH...
       eapply wf_ctx_subst_cb...
-  - Case "typing_tapp".
-    assert (Ifx0 : (if x0 == x then (var_f u) else (var_f x0)) = var_f (if x0 == x then u else x0))
-      by (destruct_if; reflexivity).
+  - assert (Ifx0 : (if x0 == x then (var_f u) else (var_f x0)) = var_f (if x0 == x then u else x0))
+      by (destruct (x0 == x); eauto).
     rewrite Ifx0.
     rewrite subst_ct_open_tt...
     eapply typing_tapp with (Q := subst_ct x (cse_fvar u) Q) (C := subst_cse x (cse_fvar u) C0) (x := (if x0 == x then u else x0)).
@@ -380,9 +360,8 @@ Proof with eauto*.
       rewrite <- Ifx0.
       eapply IHTyp...
     + apply sub_through_subst_ct with (CU := C) (U := R)...
-  - Case "typing_box".
-    assert (Ifx0 : (if x0 == x then (var_f u) else (var_f x0)) = var_f (if x0 == x then u else x0))
-      by (destruct_if; reflexivity).
+  - assert (Ifx0 : (if x0 == x then (var_f u) else (var_f x0)) = var_f (if x0 == x then u else x0))
+      by (destruct (x0 == x); eauto).
     rewrite Ifx0.
     eapply typing_box.
     + replace (subst_cse x (cse_fvar u) C0 # subst_ct x (cse_fvar u) R0)
@@ -391,9 +370,8 @@ Proof with eauto*.
       rewrite <- Ifx0.
       eapply IHTyp...
     + apply (wf_cse_over_subst Γ Δ (C # R) x (cse_fvar u) C0)...
-  - Case "typing_unbox".
-    assert (Ifx0 : (if x0 == x then (var_f u) else (var_f x0)) = var_f (if x0 == x then u else x0))
-      by (destruct_if; reflexivity).
+  - assert (Ifx0 : (if x0 == x then (var_f u) else (var_f x0)) = var_f (if x0 == x then u else x0))
+      by (destruct (x0 == x); eauto).
     rewrite Ifx0.
     apply typing_unbox.
     + replace ({} # (□ subst_cse x (cse_fvar u) C0 # subst_ct x (cse_fvar u) R0))
@@ -405,9 +383,7 @@ Proof with eauto*.
       rewrite <- Ifx0.
       eapply IHTyp...
     + eapply wf_cse_over_subst...
-  - Case "typing_sub".
-    Set Printing Coercions.
-    apply typing_sub with (R := subst_ct x (cse_fvar u) R0).
+  - apply typing_sub with (R := subst_ct x (cse_fvar u) R0).
     + eapply IHTyp...
     + apply sub_through_subst_ct with (CU := C) (U := R)...
 Qed.
@@ -421,12 +397,12 @@ Proof with eauto 3.
   dependent induction WfTyp; simpl in *...
   - apply binds_In in H.
     fsetdec.
-  - pick fresh y for (L `u`A dom Γ `u`A {x}A).
+  - pick fresh y for (L `union`A dom Γ `union`A {{ x }}A).
     specialize (H0 y ltac:(fsetdec) ltac:(fsetdec)).
     apply notin_fv_tt_open_ct in H0.
     specialize (IHWfTyp Dom).
     fsetdec.
-  - pick fresh y for (L `u`A dom Γ `u`A {x}A).
+  - pick fresh y for (L `union`A dom Γ `union`A {{ x }}A).
     specialize (H1 y ltac:(fsetdec) ltac:(fsetdec)).
     apply notin_fv_tt_open_tt in H1.
     specialize (IHWfTyp Dom).
@@ -460,32 +436,27 @@ Proof with simpl_env;
     inversion WfCtx...
   }
   assert (ZNotInDomΓ : Z ∉ dom Γ).
-  { eapply fresh_mid_tail, ok_from_wf_ctx.
+  { eapply fresh_mid_tail, uniq_from_wf_ctx.
     applys typing_regular Typ.
   }
   remember (Δ ++ [(Z, bind_sub Q)] ++ Γ).
   generalize dependent Δ.
   induction Typ; intros Δ EQ; subst;
     simpl subst_te in *; simpl subst_tt in *.
-  - Case "typing_var".
-    rename select (binds _ _ _) into Binds.
-    binds_cases Binds.
-    + SCase "x ∈ dom Γ".
-      rewrite <- subst_tt_fresh.
-      * apply typing_var with (C := C)...
-      * apply notin_fv_wf_typ with (Γ := Γ) (S := S)...
-        apply wf_typ_from_binds_typ with (S := S) in H1.
-        inversion H1; subst...
-        applys sub_regular PsubQ.
-    + SCase "x ∈ dom Δ".
-      apply typing_var with (C := C)...
+  - rename select (binds _ _ _) into Binds.
+    analyze_binds Binds.
+    + apply typing_var with (C := C)...
       replace (bind_typ (C # subst_tt Z P R))
          with (subst_tb Z P (bind_typ (C # R)))
            by reflexivity.
-      apply binds_head, binds_map.
+      apply binds_app_2, binds_map.
       assumption.
-  - Case "typing_abs".
-    replace (exp_cv e1)
+    + rewrite <- subst_tt_fresh.
+      * apply typing_var with (C := C)...
+      * apply notin_fv_wf_typ with (Γ := Γ) (S := S)...
+        apply wf_typ_from_binds_typ with (S := S) in BindsTac0...
+        inversion BindsTac0; subst...
+  - replace (exp_cv e1)
        with (exp_cv (subst_te Z P e1))
          by (symmetry; apply subst_te_fresh_exp_cv).
     pick fresh x and apply typing_abs.
@@ -501,21 +472,16 @@ Proof with simpl_env;
       assumption.
       apply wf_ctx_typ...
       reflexivity.
-  - Case "typing_app".
-    assert (Z <> x).
+  - assert (Z <> x).
     { destruct (typing_var_implies_binds_typ _ _ _ _ _ Typ2) as [C' [R' [Binds _]]].
-      binds_cases Binds; simpl_env in *...
-      assert (Z ∉ dom Δ) by (eapply fresh_mid_head; eauto* ).
-      apply binds_In in H0.
-      fsetdec.
+      assert (Z ∉ dom Δ) by (eapply fresh_mid_head; eauto ).
+      analyze_binds Binds; rename select (binds _ _ _) into Binds; apply binds_In in Binds; fsetdec.
     }
     simpl.
     replace (subst_tt Z P (open_ct T (cse_fvar x)))
        with (open_ct (subst_tt Z P T) (cse_fvar x))
-         by (apply open_ct_subst_tt; eauto* )...
-    eapply typing_app...
-    - Case "typing_let".
-      pick fresh y and apply typing_let...
+         by (apply open_ct_subst_tt; eauto )...
+    - pick fresh y and apply typing_let...
       rewrite <- subst_te_open_ve...
       rewrite_env (map (subst_tb Z P) ([(y, bind_typ (C1 # R1))] ++ Δ) ++ Γ).
       apply H0.
@@ -524,8 +490,7 @@ Proof with simpl_env;
       2: reflexivity.
       assert (WfC1R1 : wf_typ (Δ ++ [(Z, bind_sub Q)] ++ Γ) S (C1 # R1)) by applys typing_regular Typ.
       apply wf_ctx_typ...
-  - Case "typing_tabs".
-    replace (exp_cv e1)
+  - replace (exp_cv e1)
        with (exp_cv (subst_te Z P e1))
          by (symmetry; apply subst_te_fresh_exp_cv).
     pick fresh Y and apply typing_tabs.
@@ -539,30 +504,26 @@ Proof with simpl_env;
       assumption.
       2: reflexivity.
       apply wf_ctx_sub...
-  - Case "typing_tapp".
-    rewrite subst_tt_open_tt...
-  - Case "typing_box".
-    apply typing_box...
+  - rewrite subst_tt_open_tt...
+  - apply typing_box...
     assert (WfCR : wf_typ (Δ ++ [(Z, bind_sub Q)] ++ Γ) S (C # R)).
     { applys typing_regular Typ. }
     assert (WfC : wf_cse (Δ ++ [(Z, bind_sub Q)] ++ Γ) S C).
     { inversion WfCR... }
 
     apply (wf_cse_subst_tb _ _ Q Z P C)...
-  - Case "typing_unbox".
-    apply typing_unbox...
+  - apply typing_unbox...
     eapply wf_cse_subst_tb...
-  - Case "typing_sub".
-    eapply typing_sub...
+  - eapply typing_sub...
     apply sub_reflexivity...
 Qed.
 
 Lemma typing_through_open_ve_typing : forall Γ S (x y : atom) U e T,
-  y ∉ (fv_ct T `u`A fv_ve e `u`A fv_ce e) ->
+  y ∉ (fv_ct T `union`A fv_ve e `union`A fv_ce e) ->
   typing ([(y, bind_typ U)] ++ Γ) S (open_ve e y (cse_fvar y)) T ->
   typing Γ S x U ->
   typing Γ S (open_ve e x (cse_fvar x)) T.
-Proof with eauto*.
+Proof with eauto.
   intros * NotIn Typ xTyp.
   assert (WfCtx : wf_ctx ([(y, bind_typ U)] ++ Γ) S) by applys typing_regular Typ.
   inversion WfCtx; subst.
@@ -586,11 +547,11 @@ Proof with eauto*.
 Qed.
 
 Lemma typing_through_open_ve_typing_open : forall Γ S (x y : atom) U e T,
-  y ∉ (fv_ct T `u`A fv_ve e `u`A fv_ce e) ->
+  y ∉ (fv_ct T `union`A fv_ve e `union`A fv_ce e) ->
   typing ([(y, bind_typ U)] ++ Γ) S (open_ve e y (cse_fvar y)) (open_ct T (cse_fvar y)) ->
   typing Γ S x U ->
   typing Γ S (open_ve e x (cse_fvar x)) (open_ct T (cse_fvar x)).
-Proof with eauto*.
+Proof with eauto.
   intros * NotIn Typ xTyp.
   assert (WfCtx : wf_ctx ([(y, bind_typ U)] ++ Γ) S) by applys typing_regular Typ.
   inversion WfCtx; subst.
@@ -614,11 +575,11 @@ Proof with eauto*.
 Qed.
 
 Lemma typing_through_open_te : forall Γ S (Y : atom) e T P Q,
-  Y ∉ (fv_tt T `u`A fv_ct T `u`A fv_te e `u`A fv_ce e) ->
+  Y ∉ (fv_tt T `union`A fv_ct T `union`A fv_te e `union`A fv_ce e) ->
   typing ([(Y, bind_sub Q)] ++ Γ) S (open_te e Y) (open_tt T Y) ->
   sub Γ S P Q ->
   typing Γ S (open_te e P) (open_tt T P).
-Proof with eauto*.
+Proof with eauto.
   intros * NotIn Typ Sub.
   rewrite_env (map (subst_tb Y P) ∅ ++ Γ).
   replace (open_te e P)
